refine the model and prove thm about PC

model/agp32RelationScript.sml
@@ -18,7 +18,7 @@ Definition enable_stg_def:
   if k = 1 then s.IF.IF_PC_write_enable
   else if k = 2 then s.ID.ID_ID_write_enable
   else if k = 3 then s.ID.ID_EX_write_enable
-  else if k = 4 then (s.EX.EX_write_enable /\ s.MEM.MEM_state_flag) \/ s.MEM.MEM_enable
+  else if k = 4 then s.MEM.MEM_state_flag \/ s.MEM.MEM_enable
   else if k = 5 then (s.MEM.MEM_write_enable /\ s.WB.WB_state_flag) \/ s.WB.WB_enable
   else F
 End
@@ -73,8 +73,8 @@ Definition Init_def:
   (s.EX.EX_PC_sel = 0w) /\
   ~s.EX.EX_jump_sel /\
   (s.EX.EX_opc = 15w) /\
-  ~s.EX.EX_write_enable /\
   (s.MEM.MEM_opc = 15w) /\
+  ~s.MEM.MEM_state_flag /\
   ~s.MEM.MEM_enable /\
   ~s.MEM.MEM_write_reg /\
   ~s.MEM.MEM_write_enable /\
