model/compilation/agp32VerilogScript.sml
@@ -12,7 +12,7 @@ local
                 "data_addr", "data_wdata", "data_wstrb"]
  val comms = ["data_out", "command", "data_addr", "data_wdata", "data_wstrb",
               "acc_arg", "acc_arg_ready", "acc_res", "acc_res_ready", "interrupt_req",
-              "PC", "ID_PC", "EX_PC", "EX_imm", "EX_write_enable", "EX_addrW", "EX_opc",
+              "PC", "ID_PC", "EX_PC", "EX_imm", "EX_addrW", "EX_opc",
               "MEM_PC", "MEM_dataA", "MEM_dataB", "MEM_ALU_res",
               "MEM_SHIFT_res", "MEM_write_enable", "MEM_addrW", "MEM_opc",
               "WB_write_reg", "WB_addrW", "MEM_enable", "WB_enable"]
